src/klas/Klas.SDPA.LSE.fst
@@ -1,4 +1,4 @@
-module Klas.Attention
+module Klas.SDPA.LSE
 
 #lang-pulse
 open Kuiper
@@ -9,14 +9,14 @@ open Kuiper.Tensor
 open Kuiper.Index
 open Kuiper.Bijection
 
-open Kuiper.Kernel.Attention
+open Kuiper.Kernel.SDPA.LSE
 module SZ = Kuiper.SizeT
 
-let sdpa_naive_bf16
+let sdpa_lse_naive_bf16
   (n h: szp) 
   (l s: szp) 
   (e ev: szp { SZ.fits (n * h * l * e) /\ SZ.fits (n * h * s * e) /\ SZ.fits (n * h * s * ev) /\ SZ.fits (n * h * l * s) }) = 
-  sdpa_naive #bf16 n h l s e ev 
+  sdpa_lse_naive #bf16 n h l s e ev 
   #(l4_batched_row_major n h l e)
   #(l4_batched_row_major n h s e)
   #(l4_batched_row_major n h s ev)
